repatch/repatch2_generated.c
@@ -98,7 +98,7 @@ static unsigned int get_sub(unsigned int x, unsigned int y)
 
 static unsigned int get_addr_ofs(unsigned long long x, int ofs)
 {
-  return (unsigned int) (x + (unsigned long long) ofs);
+  return (unsigned int) (x + (unsigned long long) (unsigned int) ofs);
 }
 
 static _Bool is_well_chunk_bool(unsigned int chunk)
