src/DxState.v
@@ -13,8 +13,8 @@ Import ListNotations.
 Record state := mkst {
   pc_loc  : sint32_t;  (**r should pc_loc be u32 or s32: because ofs is s16, res = pc_loc+ofs may be negative! we should test res before calculating *)
   flag    : bpf_flag;
-  mem_num : uint32_t;  (**r number of memory regions *)
   regs_st : regmap;
+  mrs_num : nat;  (**r number of memory regions, put it here to guarantee align *)
   bpf_mrs : MyMemRegionsType;
   bpf_m   : Memory.mem;
 }.
@@ -24,8 +24,8 @@ Definition init_mem: Memory.mem := Memory.Mem.empty.
 Definition init_state: state := {|
   pc_loc  := Int.zero;
   flag    := BPF_OK;
-  mem_num := Int.zero;
   regs_st := init_regmap;
+  mrs_num := 0;
   bpf_mrs := default_memory_regions;
   bpf_m   := init_mem;
  |}.
@@ -35,8 +35,8 @@ Definition eval_pc (st: state): sint32_t := pc_loc st.
 Definition upd_pc (p: sint32_t) (st:state): state := {|
   pc_loc  := p;
   flag    := flag st;
-  mem_num := mem_num st;
   regs_st := regs_st st;
+  mrs_num := mrs_num st;
   bpf_mrs := bpf_mrs st;
   bpf_m   := bpf_m st;
 |}.
@@ -44,8 +44,8 @@ Definition upd_pc (p: sint32_t) (st:state): state := {|
 Definition upd_pc_incr (st:state): state := {|
   pc_loc  := Int.add (pc_loc st) Int.one;
   flag    := flag st;
-  mem_num := mem_num st;
   regs_st := regs_st st;
+  mrs_num := mrs_num st;
   bpf_mrs := bpf_mrs st;
   bpf_m   := bpf_m st;
 |}.
@@ -55,13 +55,13 @@ Definition eval_flag (st:state): bpf_flag := flag st.
 Definition upd_flag (f: bpf_flag) (st:state): state := {|
   pc_loc  := pc_loc st;
   flag    := f;
-  mem_num := mem_num st;
   regs_st := regs_st st;
+  mrs_num := mrs_num st;
   bpf_mrs := bpf_mrs st;
   bpf_m   := bpf_m st;
 |}.
 
-Definition eval_mem_num (st:state): nat := Z.to_nat (Int.unsigned (mem_num st)). (**r uint32_t -> nat*)
+Definition eval_mem_num (st:state): nat := (mrs_num st). (**r uint32_t -> nat*)
 
 (*
 Definition upd_mem_num_incr (st:state): state := {|
@@ -79,8 +79,8 @@ Definition eval_reg (r: reg) (st:state): val64_t :=
 Definition upd_reg (r:reg) (v:val64_t) (st:state): state := {|
   pc_loc  := pc_loc st;
   flag    := flag st;
-  mem_num := mem_num st;
   regs_st := upd_regmap r v (regs_st st);
+  mrs_num := mrs_num st;
   bpf_mrs := bpf_mrs st;
   bpf_m   := bpf_m st;
 |}.
@@ -110,8 +110,8 @@ Definition eval_mem (st: state):Mem.mem := bpf_m st.
 Definition upd_mem (m: Mem.mem) (st: state): state := {| (**r never be used I guess *)
   pc_loc  := pc_loc st;
   flag    := flag st;
-  mem_num := mem_num st;
   regs_st := regs_st st;
+  mrs_num := mrs_num st;
   bpf_mrs := bpf_mrs st;
   bpf_m   := m;
 |}.
@@ -146,7 +146,7 @@ Definition store_mem_reg (chunk: memory_chunk) (ptr: valu32_t) (v: val64_t) (st:
 Definition state_struct_type: Ctypes.type := Ctypes.Tstruct state_id Ctypes.noattr.
 
 Definition state_struct_def: Ctypes.composite_definition := 
-  Ctypes.Composite state_id Ctypes.Struct [(pc_id, C_U32); (flag_id, C_S32); (mem_num_id, C_U32); (regmaps_id, C_regmap); (mem_regs_id, mem_region_type)] Ctypes.noattr.
+  Ctypes.Composite state_id Ctypes.Struct [(pc_id, C_U32); (flag_id, C_S32); (regmaps_id, C_regmap); (mem_regs_id, mem_region_type); (mem_num_id, C_U32)] Ctypes.noattr.
 
 Definition stateCompilableType := MkCompilableType state state_struct_type.
 
