benchmark/proof/correct_upd_flag.v
@@ -1,0 +1,104 @@
+From bpf.src Require Import DxIntegers DxValues DxMemRegion DxState DxMonad DxFlag DxInstructions.
+From Coq Require Import List Lia ZArith.
+From compcert Require Import Integers Values Clight Memory.
+Import ListNotations.
+
+From bpf.proof Require Import Clightlogic MatchState CorrectRel CommonLemma.
+From bpf.benchmark Require Import clightlogicexample.
+
+(**
+
+static void upd_flag(struct bpf_state* st, int f){
+  ( *st).bpf_flag = f;
+  return ;
+}
+
+Definition upd_flag (f:bpf_flag) : M unit := fun st => Some (tt, upd_flag f st).
+*)
+
+Section Upd_flag.
+
+  (** The program contains our function of interest [fn] *)
+  Definition p : Clight.program := prog.
+
+  (* [Args,Res] provides the mapping between the Coq and the C types *)
+  (* Definition Args : list CompilableType := [stateCompilableType].*)
+  Definition args : list Type := [(bpf_flag:Type)].
+  Definition res : Type := unit.
+
+  (* [f] is a Coq Monadic function with the right type *)
+  Definition f : arrow_type args (M res) := DxMonad.upd_flag.
+
+  Variable state_block: block. (**r a block storing all rbpf state information? *)
+
+  (* [fn] is the Cligth function which has the same behaviour as [f] *)
+  Definition fn: Clight.function := f_upd_flag.
+
+  Definition modifies : list block := [state_block]. (* of the C code *)
+
+  Definition stateM_correct (st:unit) (v: val) (stm:stateM) (m: Memory.Mem.mem) :=
+    v = Vptr state_block Ptrofs.zero /\ match_state state_block stm m.
+
+  (* [match_arg] relates the Coq arguments and the C arguments *)
+  Definition match_arg_list : DList.t (fun x => x -> val -> stateM -> Memory.Mem.mem -> Prop) ((unit:Type) ::args) :=
+    DList.DCons stateM_correct
+                (DList.DCons (stateless flag_correct)
+                             (DList.DNil _)).
+
+  (* [match_res] relates the Coq result and the C result *)
+  Definition match_res : res -> val -> stateM -> Memory.Mem.mem -> Prop := fun x v st m => True.
+
+  Instance correct_function3_upd_flag : correct_function3 p args res f fn modifies false match_arg_list match_res.
+  Proof.
+    correct_function_from_body.
+    correct_body.
+    repeat intro.
+    unfold INV in H.
+    get_invariant_more _st.
+    get_invariant_more _f.
+    unfold stateM_correct in H1.
+    unfold stateless, flag_correct in H3.
+    destruct H1 as (Hv_eq & Hst).
+    subst v v0.
+
+    simpl in c.
+    apply (upd_flags_store _ _ _ (int_of_flag c)) in Hst as Hstore.
+    destruct Hstore as (m1 & Hstore).
+    (** we need to get the value of flag in the memory *)
+    destruct Hst; clear minj mpc mregs mperm.
+    unfold Mem.loadv in mflags.
+    unfold size_of_regs in mflags; simpl in mflags.
+    
+    (** pc \in [ (state_block,0), (state_block,8) ) *)
+    (**according to the type:
+         static void upd_flag(struct bpf_state* st, int f)
+       1. return value should be Vundef
+       2. the memory is m_flag
+      *)
+    exists Vundef, m1, Events.E0.
+
+    repeat split; unfold step2.
+    - (* goal: Smallstep.star  _ _ (State _ (Ssequence ... *)
+      apply Smallstep.plus_star.
+      repeat forward_clight.
+
+      reflexivity.
+    - simpl.
+      constructor.
+    -
+      unfold unmodifies_effect.
+      intros.
+      destruct (Pos.eq_dec state_block b).
+      subst b.
+      exfalso.
+      apply H1.
+      left; reflexivity.
+      apply POrderedType.PositiveOrder.neq_sym in n.
+      symmetry.
+      apply (Mem.load_store_other AST.Mint32 m _ _ _ m1 Hstore chk _ _).
+      left; assumption.
+  Qed.
+
+End Upd_flag.
+
+Existing  Instance correct_function3_upd_flag.
